WIP

compiler/lucky13_split_full_log.ec
@@ -1,6 +1,8 @@
 require import AllCore IntDiv CoreMap List.
 from Jasmin require import JModel.
 
+require import Array128.
+require import WArray128.
 
 
 
@@ -18,6 +20,25 @@ module M = {
     leakages <- LeakAddr([]) :: leakages;
     aux <- (result `|>>` (W8.of_int 31));
     result <- aux;
+    return (result);
+  }
+  
+  proc duplicate_msb_to_all_8_jasmin (x:W32.t) : W8.t = {
+    var aux_0: W8.t;
+    var aux: W32.t;
+    
+    var result:W8.t;
+    var temp:W32.t;
+    
+    leakages <- LeakAddr([]) :: leakages;
+    aux <- x;
+    temp <- aux;
+    leakages <- LeakAddr([]) :: leakages;
+    aux <@ duplicate_msb_to_all_jasmin (temp);
+    temp <- aux;
+    leakages <- LeakAddr([]) :: leakages;
+    aux <- temp;
+    result <- (truncateu8 aux);
     return (result);
   }
   
@@ -58,6 +79,28 @@ module M = {
     return (result);
   }
   
+  proc constant_time_eq_8_jasmin (a:W32.t, b:W32.t) : W8.t = {
+    var aux_0: W8.t;
+    var aux: W32.t;
+    
+    var result:W8.t;
+    var temp:W32.t;
+    
+    leakages <- LeakAddr([]) :: leakages;
+    aux <- a;
+    temp <- aux;
+    leakages <- LeakAddr([]) :: leakages;
+    aux <- (temp `^` b);
+    temp <- aux;
+    leakages <- LeakAddr([]) :: leakages;
+    aux <- (temp - (W32.of_int 1));
+    temp <- aux;
+    leakages <- LeakAddr([]) :: leakages;
+    aux_0 <@ duplicate_msb_to_all_8_jasmin (temp);
+    result <- aux_0;
+    return (result);
+  }
+  
   proc rotate_offset_div (md_size:W32.t, div_spoiler:W32.t, mac_start:W32.t,
                           scan_start:W32.t) : W32.t = {
     var aux: W32.t;
@@ -85,60 +128,84 @@ module M = {
     return (rotate_offset);
   }
   
-  proc rotate_mac_cache (md_size:W32.t, rotate_offset:W32.t, out:W64.t,
-                         rotated_mac:W64.t) : unit = {
-    var aux_1: W8.t;
+  proc rotate_mac (md_size:W32.t, rotate_offset:W32.t, out:W64.t,
+                   rotated_mac:W8.t Array128.t) : unit = {
+    var aux_0: W8.t;
     var aux: W32.t;
-    var aux_0: W64.t;
+    var aux_1: W64.t;
     
-    var j:W32.t;
     var i:W32.t;
-    var temp:W64.t;
+    var j:W32.t;
     var temp_8:W8.t;
+    var temp:W64.t;
+    var temp2_8:W8.t;
+    var temp_32:W32.t;
     
-    leakages <- LeakAddr([]) :: leakages;
-    aux <- (W32.of_int 0);
-    j <- aux;
     leakages <- LeakAddr([]) :: leakages;
     aux <- (W32.of_int 0);
     i <- aux;
+    leakages <- LeakAddr([]) :: leakages;
+    aux <- (W32.of_int 0);
+    j <- aux;
     
     leakages <- LeakCond((i \ult md_size)) :: LeakAddr([]) :: leakages;
     
     while ((i \ult md_size)) {
-      leakages <- LeakAddr([]) :: leakages;
-      aux_0 <- (zeroextu64 rotate_offset);
-      temp <- aux_0;
-      leakages <- LeakAddr([(((W64.to_uint (rotated_mac + temp))) %/ 64)]) :: leakages;
-      aux_1 <- (loadW8 Glob.mem (W64.to_uint (rotated_mac + temp)));
-      temp_8 <- aux_1;
+      
+      leakages <- LeakCond((j \ult md_size)) :: LeakAddr([]) :: leakages;
+      
+      while ((j \ult md_size)) {
+        leakages <- LeakAddr([]) :: leakages;
+        aux_0 <@ constant_time_eq_8_jasmin (j, rotate_offset);
+        temp_8 <- aux_0;
+        leakages <- LeakAddr([]) :: leakages;
+        aux_1 <- (zeroextu64 i);
+        temp <- aux_1;
+        leakages <- LeakAddr([(W64.to_uint temp)]) :: leakages;
+        aux_0 <- (temp_8 `&` rotated_mac.[(W64.to_uint temp)]);
+        temp_8 <- aux_0;
+        leakages <- LeakAddr([]) :: leakages;
+        aux_1 <- (zeroextu64 j);
+        temp <- aux_1;
+        leakages <- LeakAddr([(W64.to_uint (out + temp))]) :: leakages;
+        aux_0 <- (loadW8 Glob.mem (W64.to_uint (out + temp)));
+        temp2_8 <- aux_0;
+        leakages <- LeakAddr([]) :: leakages;
+        aux_0 <- (temp2_8 `|` temp_8);
+        temp2_8 <- aux_0;
+        leakages <- LeakAddr([]) :: leakages;
+        aux_0 <- temp2_8;
+        leakages <- LeakAddr([(W64.to_uint (out + temp))]) :: leakages;
+        Glob.mem <- storeW8 Glob.mem (W64.to_uint (out + temp)) aux_0;
+        leakages <- LeakAddr([]) :: leakages;
+        aux <- (j + (W32.of_int 1));
+        j <- aux;
+      leakages <- LeakCond((j \ult md_size)) :: LeakAddr([]) :: leakages;
+      
+      }
       leakages <- LeakAddr([]) :: leakages;
       aux <- (rotate_offset + (W32.of_int 1));
       rotate_offset <- aux;
       leakages <- LeakAddr([]) :: leakages;
-      aux_0 <- (zeroextu64 j);
-      temp <- aux_0;
+      aux <@ constant_time_lt_jasmin (rotate_offset, md_size);
+      temp_32 <- aux;
       leakages <- LeakAddr([]) :: leakages;
-      aux_1 <- temp_8;
-      leakages <- LeakAddr([(((W64.to_uint (out + temp))) %/ 64)]) :: leakages;
-      Glob.mem <- storeW8 Glob.mem (W64.to_uint (out + temp)) aux_1;
-      leakages <- LeakAddr([]) :: leakages;
-      aux <- (j + (W32.of_int 1));
-      j <- aux;
-      leakages <- LeakAddr([]) :: leakages;
-      aux <- ((md_size \ule rotate_offset) ? (W32.of_int 0) : rotate_offset);
+      aux <- (rotate_offset `&` temp_32);
       rotate_offset <- aux;
       leakages <- LeakAddr([]) :: leakages;
       aux <- (i + (W32.of_int 1));
       i <- aux;
+      leakages <- LeakAddr([]) :: leakages;
+      aux <- (W32.of_int 0);
+      j <- aux;
     leakages <- LeakCond((i \ult md_size)) :: LeakAddr([]) :: leakages;
     
     }
     return ();
   }
   
-  proc ssl3_cbc_copy_mac_jasmin_cache (out:W64.t, rec:W64.t, orig_len:W32.t,
-                                       md_size:W32.t, rotated_mac:W64.t) : unit = {
+  proc ssl3_cbc_copy_mac_jasmin (out:W64.t, rec:W64.t, orig_len:W32.t,
+                                 md_size:W32.t) : unit = {
     var aux_1: W8.t;
     var aux_0: W32.t;
     var aux: W64.t;
@@ -150,6 +217,7 @@ module M = {
     var temp_32:W32.t;
     var i:W32.t;
     var temp:W64.t;
+    var rotated_mac:W8.t Array128.t;
     var j:W32.t;
     var temp2_32:W32.t;
     var mac_started:W8.t;
@@ -159,11 +227,11 @@ module M = {
     var temp2_8:W8.t;
     var div_spoiler:W32.t;
     var rotate_offset:W32.t;
-    
-    leakages <- LeakAddr([(((W64.to_uint (rec + (W64.of_int 16)))) %/ 64)]) :: leakages;
+    rotated_mac <- witness;
+    leakages <- LeakAddr([(W64.to_uint (rec + (W64.of_int 16)))]) :: leakages;
     aux <- (loadW64 Glob.mem (W64.to_uint (rec + (W64.of_int 16))));
     data <- aux;
-    leakages <- LeakAddr([(((W64.to_uint (rec + (W64.of_int 4)))) %/ 64)]) :: leakages;
+    leakages <- LeakAddr([(W64.to_uint (rec + (W64.of_int 4)))]) :: leakages;
     aux_0 <- (loadW32 Glob.mem (W64.to_uint (rec + (W64.of_int 4))));
     mac_end <- aux_0;
     leakages <- LeakAddr([]) :: leakages;
@@ -203,9 +271,9 @@ module M = {
       aux <- (zeroextu64 i);
       temp <- aux;
       leakages <- LeakAddr([]) :: leakages;
-      aux <- (W64.of_int 0);
-      leakages <- LeakAddr([(((W64.to_uint (rotated_mac + temp))) %/ 64)]) :: leakages;
-      Glob.mem <- storeW64 Glob.mem (W64.to_uint (rotated_mac + temp)) aux;
+      aux_1 <- (W8.of_int 0);
+      leakages <- LeakAddr([(W64.to_uint temp)]) :: leakages;
+      rotated_mac.[(W64.to_uint temp)] <- aux_1;
       leakages <- LeakAddr([]) :: leakages;
       aux_0 <- (i + (W32.of_int 1));
       i <- aux_0;
@@ -246,7 +314,7 @@ module M = {
       leakages <- LeakAddr([]) :: leakages;
       aux <- (zeroextu64 i);
       temp <- aux;
-      leakages <- LeakAddr([(((W64.to_uint (data + temp))) %/ 64)]) :: leakages;
+      leakages <- LeakAddr([(W64.to_uint (data + temp))]) :: leakages;
       aux_1 <- (loadW8 Glob.mem (W64.to_uint (data + temp)));
       b <- aux_1;
       leakages <- LeakAddr([]) :: leakages;
@@ -264,16 +332,16 @@ module M = {
       leakages <- LeakAddr([]) :: leakages;
       aux <- (zeroextu64 j);
       temp <- aux;
-      leakages <- LeakAddr([(((W64.to_uint (rotated_mac + temp))) %/ 64)]) :: leakages;
-      aux_1 <- (loadW8 Glob.mem (W64.to_uint (rotated_mac + temp)));
+      leakages <- LeakAddr([(W64.to_uint temp)]) :: leakages;
+      aux_1 <- rotated_mac.[(W64.to_uint temp)];
       temp2_8 <- aux_1;
       leakages <- LeakAddr([]) :: leakages;
       aux_1 <- (temp2_8 `|` temp_8);
       temp2_8 <- aux_1;
       leakages <- LeakAddr([]) :: leakages;
       aux_1 <- temp2_8;
-      leakages <- LeakAddr([(((W64.to_uint (rotated_mac + temp))) %/ 64)]) :: leakages;
-      Glob.mem <- storeW8 Glob.mem (W64.to_uint (rotated_mac + temp)) aux_1;
+      leakages <- LeakAddr([(W64.to_uint temp)]) :: leakages;
+      rotated_mac.[(W64.to_uint temp)] <- aux_1;
       leakages <- LeakAddr([]) :: leakages;
       aux_0 <- (j + (W32.of_int 1));
       j <- aux_0;
@@ -296,7 +364,44 @@ module M = {
     aux_0 <@ rotate_offset_div (md_size, div_spoiler, mac_start, scan_start);
     rotate_offset <- aux_0;
     leakages <- LeakAddr([]) :: leakages;
-    rotate_mac_cache (md_size, rotate_offset, out, rotated_mac);
+    aux <- (W64.of_int 0);
+    temp <- aux;
+    
+    leakages <- LeakCond(((truncateu32 temp) \ult md_size)) :: LeakAddr(
+    []) :: leakages;
+    
+    while (((truncateu32 temp) \ult md_size)) {
+      leakages <- LeakAddr([]) :: leakages;
+      aux_1 <- (W8.of_int 0);
+      leakages <- LeakAddr([(W64.to_uint (out + temp))]) :: leakages;
+      Glob.mem <- storeW8 Glob.mem (W64.to_uint (out + temp)) aux_1;
+      leakages <- LeakAddr([]) :: leakages;
+      aux <- (temp + (W64.of_int 1));
+      temp <- aux;
+    leakages <- LeakCond(((truncateu32 temp) \ult md_size)) :: LeakAddr(
+    []) :: leakages;
+    
+    }
+    leakages <- LeakAddr([]) :: leakages;
+    aux_0 <- md_size;
+    temp_32 <- aux_0;
+    leakages <- LeakAddr([]) :: leakages;
+    aux_0 <- (temp_32 - rotate_offset);
+    temp_32 <- aux_0;
+    leakages <- LeakAddr([]) :: leakages;
+    aux_0 <- temp_32;
+    rotate_offset <- aux_0;
+    leakages <- LeakAddr([]) :: leakages;
+    aux_0 <@ constant_time_lt_jasmin (rotate_offset, md_size);
+    temp_32 <- aux_0;
+    leakages <- LeakAddr([]) :: leakages;
+    aux <- (zeroextu64 temp_32);
+    temp <- aux;
+    leakages <- LeakAddr([]) :: leakages;
+    aux_0 <- (rotate_offset `&` (truncateu32 temp));
+    rotate_offset <- aux_0;
+    leakages <- LeakAddr([]) :: leakages;
+    rotate_mac (md_size, rotate_offset, out, rotated_mac);
     return ();
   }
 }.
