compiler/lucky13_split_full_log_proof.ec
@@ -1,0 +1,67 @@
+require import AllCore IntDiv CoreMap List.
+from Jasmin require import JModel.
+
+require import Array128 WArray128 Lucky13_split_full_log.
+
+equiv l_constant_time_lt_jasmin : M.constant_time_lt_jasmin ~ M.constant_time_lt_jasmin :
+={M.leakages}
+==> ={M.leakages}.
+proof.
+proc; inline *; sim.
+qed.
+
+equiv l_rotate_offset_div : M.rotate_offset_div ~ M.rotate_offset_div:
+={M.leakages, md_size, scan_start} /\
+(0 <= (to_uint (mac_start - scan_start)) < 2^8){1} /\ 
+(0 <= (to_uint (mac_start - scan_start)) < 2^8){2} /\
+(16 <= to_uint md_size <= 64){1}
+==> ={M.leakages}.
+proof.
+  proc; wp; skip => />.
+admitted.
+
+op wf_rec mem (rec:W64.t) (orig_len md_size : W32.t) = 
+ let mac_end = loadW32 mem (to_uint (rec + W64.of_int 4)) in
+ to_uint md_size <= to_uint mac_end /\ 
+ 1 <= to_uint orig_len - to_uint mac_end <= 256.
+
+lemma wf_rec_cond_md_size_mac_end mem rec orig_len md_size : 
+  16 <= W32.to_uint md_size <= 64 =>
+  wf_rec mem rec orig_len md_size =>
+  let mac_end = loadW32 mem (to_uint (rec + W64.of_int 4)) in
+  if (md_size + W32.of_int 256 \ult orig_len) then 
+     0 <= to_uint (mac_end - md_size - (orig_len - (md_size + W32.of_int 256))) < 256
+  else 0 <= to_uint (mac_end - md_size - W32.zero) < 256.
+proof.
+  rewrite /wf_rec /=.
+  pose mac_end := loadW32 _ _; move: mac_end => mac_end hmd [h1 [h2 h3]].
+  have -> : mac_end - md_size - (orig_len - (md_size + W32.of_int 256)) = 
+            mac_end - (orig_len - W32.of_int 256) by ring.
+  rewrite W32.ultE W32.to_uintD_small /= 1:/#.
+  case: (to_uint md_size + 256 < to_uint orig_len) => h; last first.
+  + rewrite W32.WRingA.subr0 W32.to_uintB 1:W32.uleE 1:// /#.
+  rewrite W32.to_uintB ?W32.uleE W32.to_uintB ?W32.uleE /=; smt(W32.to_uint_cmp). 
+qed.
+
+equiv l_rotate_mac_ct : M.rotate_mac ~ M.rotate_mac : ={M.leakages, out, md_size} ==> ={M.leakages}.
+proof. by proc; inline *; sim. qed.
+
+equiv l_final : M.ssl3_cbc_copy_mac_jasmin ~ M.ssl3_cbc_copy_mac_jasmin :
+={M.leakages, md_size, orig_len, out, rec} /\
+(loadW64 Glob.mem (to_uint (rec + (of_int 16)%W64))){1} = 
+(loadW64 Glob.mem (to_uint (rec + (of_int 16)%W64))){2} /\
+16 <= to_uint md_size{2} <= 64 /\
+(wf_rec Glob.mem rec orig_len md_size){1} /\ 
+(wf_rec Glob.mem rec orig_len md_size){2}  
+==> ={M.leakages}.
+proof.
+  proc.
+  call l_rotate_mac_ct; wp.
+  call l_constant_time_lt_jasmin; wp.
+  while (={M.leakages, temp, out, md_size}); 1: by sim.
+  wp => /=; conseq />.
+  call l_rotate_offset_div; wp.
+  while (={i, j, orig_len, data, md_size, M.leakages}); 1: by inline*;sim.
+  wp => /=; while (={i, md_size, M.leakages}); 1: by sim.
+  wp; skip => |> &1 &2; smt (wf_rec_cond_md_size_mac_end).
+qed.
